Fix relocation of argument `a` in `server_program`

src/Ouroboros-Mini_Protocols-Chain_Sync.thy
@@ -178,7 +178,7 @@ primrec program where
   "program Client =
     client_program point candidate_intersection_points initial_client_chain IntersectionFinding" |
   "program Server =
-    server_program point initial_server_chain 0 False server_chain_updates"
+    server_program point initial_server_chain server_chain_updates 0 False"
 
 end
 
@@ -197,7 +197,7 @@ proof
       )
   moreover
   have "
-    server_program point initial_server_chain read_pointer must_roll_back server_chain_updates
+    server_program point initial_server_chain server_chain_updates read_pointer must_roll_back
     \<Colon>\<^bsub>Server\<^esub>
     Cont possibilities"
     for read_pointer and must_roll_back
